Read after write is verified

IronFleetDefault/ironfleet/src/Dafny/Distributed/Protocol/CausalMesh/proof/read_after_write.dfy
@@ -2,6 +2,8 @@ include "../distributed_system.dfy"
 include "causalcut.dfy"
 include "packet_sending.dfy"
 include "message_read_reply.dfy"
+include "monotonic_read.dfy"
+include "monotonic_write.dfy"
 include "../../../Common/Collections/Seqs.s.dfy"
 
 module CausalMesh_Proof_Read_After_Write_i {
@@ -18,53 +20,71 @@ import opened CausalMesh_Proof_Constants_i
 import opened CausalMesh_Proof_CausalCut_i
 import opened CausalMesh_Proof_PacketSending_i
 import opened CausalMesh_Proof_MessageReadReply_i
+import opened CausalMesh_Proof_Monotonic_Read_i
+import opened CausalMesh_Proof_Monotonic_Write_i
 import opened Collections__Seqs_s
 import opened Collections__Maps_i
 import opened Collections__Maps2_s
 
-// lemma lemma_AllDepsInCCacheAfterPullDepsAreExistsInICache()
 
-predicate WriteReplyIsLargerThanVCInDeps(deps:Dependency, vc:VectorClock)
-    requires DependencyValid(deps)
-    requires VectorClockValid(vc)
-{
-    forall k :: k in deps ==> VCHappendsBefore(deps[k], vc) || VCEq(deps[k], vc)
-}
-
-predicate WriteReplyIsLargerThanVCInLocal(local:map<Key, Meta>, vc:VectorClock)
-    requires forall k :: k in local ==> MetaValid(local[k])
-    requires VectorClockValid(vc)
-{
-    forall k :: k in local ==> VCHappendsBefore(local[k].vc, vc) || VCEq(local[k].vc, vc)
-}
-
-predicate WriteReplyHasCorrspondingWriteWithSmallerVC(
-    b:Behavior<CMState>,
-    i:int,
-    p:Packet
+lemma lemma_ReadAWriteCanObserveAllItsPreviousReadsAndWrites(
+    behavior:seq<CMState>
 )
-    requires 0 < i 
-    requires IsValidBehaviorPrefix(b, i)
-    requires p in b[i].environment.sentPackets && p.msg.Message_Write_Reply? && PacketValid(p)
+    requires |behavior| > 0 
+    requires CMInit(behavior[0])
+    requires forall i :: 
+                0 <= i < |behavior| - 1 ==> CMNext(behavior[i], behavior[i+1])
+    ensures var b := ConvertBehaviorSeqToImap(behavior);
+        forall i :: 0 <= i < |behavior| ==> AllReadReplyVCIsLargerThanAllPreviousWritesReal(b, i) 
 {
-    lemma_BehaviorValidImpliesOneStepValid(b, i);
-    forall wp :: wp in b[i].environment.sentPackets && wp.msg.Message_Write?
-                    && p.msg.key_wreply == wp.msg.key_write
-                    && p.dst == wp.src
-                    ==> WriteReplyIsLargerThanVCInDeps(wp.msg.deps_write, p.msg.vc_wreply)
-                        && WriteReplyIsLargerThanVCInLocal(wp.msg.local, p.msg.vc_wreply)
+    var b := ConvertBehaviorSeqToImap(behavior);
+    if |behavior| == 1 { 
+        assert !exists p :: p in b[0].environment.sentPackets;
+        assert AllReadReplyVCIsLargerThanAllPreviousWrites(b, 0);
+        lemma_AllReadReplyVCIsLargerThanAllPreviousWrites(b, 0);
+        assert AllReadReplyVCIsLargerThanAllPreviousWritesReal(b, 0);
+    }
+    else
+    { 
+        assert forall j {:trigger CMNext(b[j], b[j+1])} :: 0 <= j < |behavior| - 1 ==> CMNext(b[j], b[j+1]); 
+        assert forall j :: 0 <= j < |behavior| - 1 ==> CMNext(b[j], b[j+1]);
+        // lemma_ReadReplyHasHigherVCThanDepsPrefix(b, |low_level_behavior| - 1);
+        lemma_ReadAfterWritePrefix(b, |behavior| - 1);
+        // assert AllReadReplyHasCorrspondingReadWithSmallOrEqVCForSameKeyInDeps(b, |low_level_behavior| - 1);
+        assert forall i :: 0 < i < |behavior| ==> AllReadReplyVCIsLargerThanAllPreviousWrites(b, i);
+        // lemma_AllReadReplyVCIsLargerThanAllPreviousWrites(b, i);
+        // assert forall i :: 0 < i < |behavior| ==> AllReadReplyVCIsLargerThanAllPreviousWritesReal(b, i);
+    }
+
+    assert forall i :: 0 <= i < |behavior| ==> AllReadReplyVCIsLargerThanAllPreviousWrites(b, i);
+    lemma_AllReadReplyVCIsLargerThanAllPreviousWritesPrefix(b, |behavior|-1);
+    assert forall i :: 0 <= i < |behavior| ==> AllReadReplyVCIsLargerThanAllPreviousWritesReal(b, i);
 }
 
-predicate AllWriteReplyHasCoorspondingWriteWithSmallerOrEqVCInDepsAndLocals(
+lemma lemma_AllReadReplyVCIsLargerThanAllPreviousWritesPrefix(
     b:Behavior<CMState>,
-    i:int
+    k:int
 )
-    requires 0 < i 
-    requires IsValidBehaviorPrefix(b, i)
+    requires k >= 0 
+    requires IsValidBehaviorPrefix(b, k)
+    // requires forall i :: 
+    //             0 <= i <= k ==> CMNext(b[i], b[i+1])
+    requires forall i :: 0 <= i <= k ==> AllReadReplyVCIsLargerThanAllPreviousWrites(b, i) 
+    ensures  forall i :: 0 <= i <= k ==> AllReadReplyVCIsLargerThanAllPreviousWritesReal(b, i) 
 {
-    lemma_BehaviorValidImpliesOneStepValid(b, i);
+    if k == 0 {
+        lemma_AllReadReplyVCIsLargerThanAllPreviousWrites(b, 0);
+        assert AllReadReplyVCIsLargerThanAllPreviousWritesReal(b, 0);
+        return;
+    }
+    lemma_AllReadReplyVCIsLargerThanAllPreviousWritesPrefix(b, k-1);
+    assert forall i :: 0 <= i <= k-1 ==> AllReadReplyVCIsLargerThanAllPreviousWritesReal(b, i);
+    
+    assert AllReadReplyVCIsLargerThanAllPreviousWrites(b, k);
+    lemma_AllReadReplyVCIsLargerThanAllPreviousWrites(b, k);
+    assert AllReadReplyVCIsLargerThanAllPreviousWritesReal(b, k);
+    assert forall i :: 0 <= i <= k ==> AllReadReplyVCIsLargerThanAllPreviousWritesReal(b, i);
 
-    forall p :: p in b[i].environment.sentPackets && p.msg.Message_Write_Reply? ==> WriteReplyHasCorrspondingWriteWithSmallerVC(b, i, p)
 }
 
 predicate ReadReplyVCIsLargerThanAllPreviousWrites(
@@ -83,79 +103,231 @@ predicate ReadReplyVCIsLargerThanAllPreviousWrites(
                 ==> WriteReplyHasCorrspondingWriteWithSmallerVC(b, i, wrp)
 }
 
-lemma lemma_WriteReplyHasHigerVCThanDepsAndLocalPrefix(
+predicate ReadReplyVCIsLargerThanAllPreviousWritesReal(
     b:Behavior<CMState>,
-    i:int
+    i:int,
+    p:Packet
 )
     requires 0 < i 
     requires IsValidBehaviorPrefix(b, i)
-    requires forall j :: 0 <= j < i ==> CMNext(b[j], b[j+1])
-    // ensures AllWriteReplyHasCoorspondingWriteWithSmallerOrEqVCInDepsAndLocals(b, i)
-    decreases i
+    requires p in b[i].environment.sentPackets && p.msg.Message_Read_Reply? && PacketValid(p)
 {
-    if i <= i {
+    lemma_BehaviorValidImpliesOneStepValid(b, i);
+    forall wrp :: wrp in b[i].environment.sentPackets && wrp.msg.Message_Write_Reply?
+            && p.msg.key_rreply == wrp.msg.key_wreply
+            && (VCHappendsBefore(wrp.msg.vc_wreply, p.msg.vc_rreply) || VCEq(wrp.msg.vc_wreply, p.msg.vc_rreply))
+                ==> exists wp :: wp in b[i].environment.sentPackets && wp.msg.Message_Write?
+                    && wrp.msg.opn_wreply == wp.msg.opn_write
+                    && wrp.msg.key_wreply == wp.msg.key_write
+                    && wrp.dst == wp.src
+                    // && WriteReplyIsLargerThanVCInDeps(wp.msg.deps_write, wrp.msg.vc_wreply)
+                    // && WriteReplyIsLargerThanVCInLocal(wp.msg.local, wrp.msg.vc_wreply)
+                    && WriteReplyIsLargerThanVCInDeps(wp.msg.deps_write, p.msg.vc_rreply)
+                    && WriteReplyIsLargerThanVCInLocal(wp.msg.local, p.msg.vc_rreply)
+}
+
+lemma lemma_VCRelationIsTransitive(
+    rrp:Packet,
+    wrp:Packet,
+    wp:Packet
+)
+    requires PacketValid(rrp)
+    requires rrp.msg.Message_Read_Reply?
+    requires PacketValid(wrp)
+    requires wrp.msg.Message_Write_Reply?
+    requires PacketValid(wp)
+    requires wp.msg.Message_Write?
+    requires (VCHappendsBefore(wrp.msg.vc_wreply, rrp.msg.vc_rreply) || VCEq(wrp.msg.vc_wreply, rrp.msg.vc_rreply))
+    requires WriteReplyIsLargerThanVCInDeps(wp.msg.deps_write, wrp.msg.vc_wreply)
+    requires WriteReplyIsLargerThanVCInLocal(wp.msg.local, wrp.msg.vc_wreply)
+    ensures WriteReplyIsLargerThanVCInDeps(wp.msg.deps_write, rrp.msg.vc_rreply)
+    ensures WriteReplyIsLargerThanVCInLocal(wp.msg.local, rrp.msg.vc_rreply)
+{
+
+}
+
+lemma lemma_ReadReplyVCIsLargerThanAllPreviousWrites(
+    b:Behavior<CMState>,
+    i:int,
+    p:Packet
+)
+    requires 0 < i 
+    requires IsValidBehaviorPrefix(b, i)
+    requires p in b[i].environment.sentPackets && p.msg.Message_Read_Reply? && PacketValid(p)
+    requires ReadReplyVCIsLargerThanAllPreviousWrites(b, i, p)
+    ensures ReadReplyVCIsLargerThanAllPreviousWritesReal(b, i, p)
+{
+    lemma_BehaviorValidImpliesOneStepValid(b, i);
+    assert forall wrp :: wrp in b[i].environment.sentPackets && wrp.msg.Message_Write_Reply?
+            && p.msg.key_rreply == wrp.msg.key_wreply
+            && (VCHappendsBefore(wrp.msg.vc_wreply, p.msg.vc_rreply) || VCEq(wrp.msg.vc_wreply, p.msg.vc_rreply))
+                ==> exists wp :: wp in b[i].environment.sentPackets && wp.msg.Message_Write?
+                    && wrp.msg.opn_wreply == wp.msg.opn_write
+                    && wrp.msg.key_wreply == wp.msg.key_write
+                    && wrp.dst == wp.src
+                    && WriteReplyIsLargerThanVCInDeps(wp.msg.deps_write, wrp.msg.vc_wreply)
+                    && WriteReplyIsLargerThanVCInLocal(wp.msg.local, wrp.msg.vc_wreply);
+    if exists wrp :: wrp in b[i].environment.sentPackets && wrp.msg.Message_Write_Reply?
+            && p.msg.key_rreply == wrp.msg.key_wreply
+            && (VCHappendsBefore(wrp.msg.vc_wreply, p.msg.vc_rreply) || VCEq(wrp.msg.vc_wreply, p.msg.vc_rreply)) {
+
+        var wrp :| wrp in b[i].environment.sentPackets && wrp.msg.Message_Write_Reply?
+                && p.msg.key_rreply == wrp.msg.key_wreply
+                && (VCHappendsBefore(wrp.msg.vc_wreply, p.msg.vc_rreply) || VCEq(wrp.msg.vc_wreply, p.msg.vc_rreply));
+        var wp :| wp in b[i].environment.sentPackets && wp.msg.Message_Write?
+                    && wrp.msg.opn_wreply == wp.msg.opn_write
+                    && wrp.msg.key_wreply == wp.msg.key_write
+                    && wrp.dst == wp.src
+                    && WriteReplyIsLargerThanVCInDeps(wp.msg.deps_write, wrp.msg.vc_wreply)
+                    && WriteReplyIsLargerThanVCInLocal(wp.msg.local, wrp.msg.vc_wreply);
+        lemma_VCRelationIsTransitive(p, wrp, wp);
+        assert ReadReplyVCIsLargerThanAllPreviousWritesReal(b, i, p);
+    }
+}
+
+predicate AllReadReplyVCIsLargerThanAllPreviousWrites(
+    b:Behavior<CMState>,
+    i:int
+)
+    requires 0 <= i 
+    requires IsValidBehaviorPrefix(b, i)
+{
+    if i == 0 then 
+        !exists p :: p in b[i].environment.sentPackets
+    else
+        lemma_BehaviorValidImpliesOneStepValid(b, i);
+        forall p :: p in b[i].environment.sentPackets && p.msg.Message_Read_Reply? ==> 
+            ReadReplyVCIsLargerThanAllPreviousWrites(b, i, p)
+}
+
+predicate AllReadReplyVCIsLargerThanAllPreviousWritesReal(
+    b:Behavior<CMState>,
+    i:int
+)
+    requires 0 <= i 
+    requires IsValidBehaviorPrefix(b, i)
+{
+    if i == 0 then 
+        !exists p :: p in b[i].environment.sentPackets
+    else
+        lemma_BehaviorValidImpliesOneStepValid(b, i);
+        forall p :: p in b[i].environment.sentPackets && p.msg.Message_Read_Reply? ==> 
+            ReadReplyVCIsLargerThanAllPreviousWritesReal(b, i, p)
+}
+
+lemma lemma_AllReadReplyVCIsLargerThanAllPreviousWrites(
+    b:Behavior<CMState>,
+    i:int
+)
+    requires 0 <= i 
+    requires IsValidBehaviorPrefix(b, i)
+    requires AllReadReplyVCIsLargerThanAllPreviousWrites(b, i)
+    ensures AllReadReplyVCIsLargerThanAllPreviousWritesReal(b, i)
+{
+    if i > 0 {
+        lemma_BehaviorValidImpliesOneStepValid(b, i);
+        if exists p :: p in b[i].environment.sentPackets && p.msg.Message_Read_Reply? {
+            var p :| p in b[i].environment.sentPackets && p.msg.Message_Read_Reply?;
+            lemma_ReadReplyVCIsLargerThanAllPreviousWrites(b, i, p);
+        }
+    }
+}
+
+lemma lemma_ReadAfterWritePrefix(
+    b:Behavior<CMState>,
+    i:int
+)
+    requires i >= 0
+    requires IsValidBehaviorPrefix(b, i)
+    requires forall j :: 0 <= j < i ==> CMNext(b[j], b[j+1])
+    ensures forall j :: 0 < j <= i ==> AllReadReplyVCIsLargerThanAllPreviousWrites(b, j)
+{
+    if i == 0 {
         return;
     }
 
     lemma_ConstantsAllConsistent(b, i-1);
     lemma_ConstantsAllConsistent(b, i);
 
-    if !StepSendsWriteReply(b[i-1], b[i]){
-        lemma_WriteReplyHasHigerVCThanDepsAndLocalPrefix(b, i-1);
+    lemma_ReadAfterWritePrefix(b, i-1);
+    lemma_MonotonicWritePrefix(b, i);
+
+    lemma_ReadReplyVCIsLargerThanAllPreviousWritesPrefix(b, i);
+    assert forall j :: 0 < j <= i ==> AllReadReplyVCIsLargerThanAllPreviousWrites(b, j);
+}
+
+
+lemma lemma_ReadReplyVCIsLargerThanAllPreviousWritesPrefix(
+    b:Behavior<CMState>,
+    i:int
+)
+    requires 0 < i 
+    requires IsValidBehaviorPrefix(b, i)
+    requires forall j :: 0 <= j < i ==> CMNext(b[j], b[j+1])
+    requires AllWriteReplyHasCoorspondingWriteWithSmallerOrEqVCInDepsAndLocalsAlways(b, i)
+    ensures AllReadReplyVCIsLargerThanAllPreviousWrites(b, i)
+{
+    if i <= 1 {
+        assert AllReadReplyVCIsLargerThanAllPreviousWrites(b, i);
         return;
     }
 
-    lemma_WriteReplyHasHigerVCThanDepsAndLocalPrefix(b, i-1);
+    lemma_ConstantsAllConsistent(b, i-1);
+    lemma_ConstantsAllConsistent(b, i);
 
-    var p :| p in b[i].environment.sentPackets && p !in b[i-1].environment.sentPackets && p.msg.Message_Write_Reply?;
+    if !StepSendsReadReply(b[i-1], b[i]){
+        lemma_ReadReplyVCIsLargerThanAllPreviousWritesPrefix(b, i-1); 
+        // assume AllReadReplyVCIsLargerThanAllPreviousWrites(b, i-1);
+        assert forall p :: p in b[i].environment.sentPackets && p.msg.Message_Read_Reply? ==> p in b[i-1].environment.sentPackets; 
+        assert CMNext(b[i-1], b[i]);
+        assert forall p :: p in b[i-1].environment.sentPackets ==> p in b[i].environment.sentPackets;
+        lemma_ReadReplyVCIsLargerThanAllPreviousWritesConstant(b, i);
+        assert AllReadReplyVCIsLargerThanAllPreviousWrites(b, i);
+        return;
+    }
+
+    lemma_ReadReplyVCIsLargerThanAllPreviousWritesPrefix(b, i-1);
+
+    var p :| p in b[i].environment.sentPackets && p !in b[i-1].environment.sentPackets && p.msg.Message_Read_Reply?;
 
     assert PacketValid(p);
+    var idx, ios := lemma_ActionThatSendsReadReplyIsServerReceiveRead(b[i-1], b[i], p);
 
-    var idx, ios := lemma_ActionThatSendsWriteReplyIsServerReceiveWrite(b[i-1], b[i], p);
+    var p_read := ios[0].r;
+    assert ReceiveRead(b[i-1].servers[idx].s, b[i].servers[idx].s, p_read, [p]);
+    assert AllWriteReplyHasCoorspondingWriteWithSmallerOrEqVCInDepsAndLocals(b, i);
 
-    var p_write := ios[0].r;
-    var sp := ExtractSentPacketsFromIos(ios);
-
-    assert ReceiveWrite(b[i-1].servers[idx].s, b[i].servers[idx].s, p_write, sp);
+    assert AllReadReplyVCIsLargerThanAllPreviousWrites(b, i);
 }
 
-predicate StepSendsWriteReply(s:CMState, s':CMState)
-    requires CMNext(s, s')
+lemma lemma_ReadReplyVCIsLargerThanAllPreviousWritesConstant(
+    b:Behavior<CMState>,
+    i:int
+)
+    requires 1 < i 
+    requires IsValidBehaviorPrefix(b, i)
+    requires AllReadReplyVCIsLargerThanAllPreviousWrites(b, i-1)
+    requires forall j :: 0 <= j < i ==> CMNext(b[j], b[j+1])
+    requires forall p :: p in b[i].environment.sentPackets && p.msg.Message_Read_Reply? ==> p in b[i-1].environment.sentPackets
+    requires forall p :: p in b[i-1].environment.sentPackets ==> p in b[i].environment.sentPackets
+    requires AllWriteReplyHasCoorspondingWriteWithSmallerOrEqVCInDepsAndLocalsAlways(b, i)
+    ensures AllReadReplyVCIsLargerThanAllPreviousWrites(b, i)
 {
-    // && s.environment.nextStep.LEnvStepHostIos?
-    && exists p :: p in s'.environment.sentPackets && p.msg.Message_Write_Reply? && p !in s.environment.sentPackets
-}
+    lemma_BehaviorValidImpliesOneStepValid(b, i);
 
-lemma lemma_ServerWriteReplyLargerVCThanLocalAndDeps(s:Server, s':Server, p:Packet, sp:seq<Packet>)
-    requires p.msg.Message_Write?
-    requires ServerValid(s)
-    requires PacketValid(p) 
-    requires ReceiveWrite(s, s', p, sp)
-    ensures |sp| == 2
-    ensures sp[0].msg.Message_Write_Reply?
-    ensures forall k :: k in p.msg.local ==> 
-                VCHappendsBefore(p.msg.local[k].vc, sp[0].msg.vc_wreply) || VCEq(p.msg.local[k].vc, sp[0].msg.vc_wreply)
-    ensures forall k :: k in p.msg.deps_write ==> 
-                VCHappendsBefore(p.msg.deps_write[k], sp[0].msg.vc_wreply) || VCEq(p.msg.deps_write[k], sp[0].msg.vc_wreply)
-{
-    assert forall k :: k in p.msg.local ==> MetaValid(p.msg.local[k]);
-    var local_metas := set m | m in p.msg.local.Values;
-    var vcs_local := set m | m in local_metas :: m.vc;
-    assert forall vc :: vc in vcs_local ==> VectorClockValid(vc); 
-    var merged_vc := FoldVC(s.gvc, vcs_local);
-    assert forall vc :: vc in vcs_local ==> VCHappendsBefore(vc, merged_vc) || VCEq(vc, merged_vc);
-    assert forall m :: m in local_metas ==> VCHappendsBefore(m.vc, merged_vc) || VCEq(m.vc, merged_vc);
-    assert forall k :: k in p.msg.local ==> p.msg.local[k] in local_metas;
-    assert forall k :: k in p.msg.local ==> 
-                VCHappendsBefore(p.msg.local[k].vc, sp[0].msg.vc_wreply) || VCEq(p.msg.local[k].vc, sp[0].msg.vc_wreply);
+    assert forall p :: p in b[i-1].environment.sentPackets && p.msg.Message_Read_Reply? ==> ReadReplyVCIsLargerThanAllPreviousWrites(b, i-1, p);
+    assert forall p :: p in b[i].environment.sentPackets && p.msg.Message_Read_Reply? ==> p in b[i-1].environment.sentPackets;
+    assert forall p :: p in b[i].environment.sentPackets && p.msg.Message_Read_Reply? ==> ReadReplyVCIsLargerThanAllPreviousWrites(b, i-1, p);
+    if !StepSendsWriteReply(b[i-1], b[i]) {
+        assert AllReadReplyVCIsLargerThanAllPreviousWrites(b, i);
+        return;
+    }
 
-    var vcs_deps := set k | k in p.msg.deps_write :: p.msg.deps_write[k];
-    var merged_vc2 := FoldVC(merged_vc, vcs_deps);
-    assert forall vc :: vc in vcs_deps ==> VCHappendsBefore(vc, merged_vc2) || VCEq(vc, merged_vc2);
-    assert forall k :: k in p.msg.deps_write ==> 
-                VCHappendsBefore(p.msg.deps_write[k], merged_vc2) || VCEq(p.msg.deps_write[k], merged_vc2);
-    assert forall k :: k in p.msg.deps_write ==> 
-                VCHappendsBefore(p.msg.deps_write[k], sp[0].msg.vc_wreply) || VCEq(p.msg.deps_write[k], sp[0].msg.vc_wreply);
+    assert StepSendsWriteReply(b[i-1], b[i]);
+    var p :| p in b[i].environment.sentPackets && p !in b[i-1].environment.sentPackets && p.msg.Message_Write_Reply?;
+    assert AllWriteReplyHasCoorspondingWriteWithSmallerOrEqVCInDepsAndLocals(b, i);
+    assert WriteReplyHasCorrspondingWriteWithSmallerVC(b, i, p);
+    assert AllReadReplyVCIsLargerThanAllPreviousWrites(b, i);
 }
 
 }
